extensionality

src/pSet_ZFC.lean
@@ -3,13 +3,61 @@ Copyright (c) 2020 The Flypitch Project. All rights reserved.
 Released under Apache 2.0 license as described in the file LICENSE.
 Author(s): Jesse Michael Han
 
-Showing that pSet is formally a model of ZFC.
+Showing that Set is formally a model of ZFC.
 -/
 
 import .zfc
 import .pSet_ordinal
 import tactic
+import .fol
 
+open fol
+local notation h :: t  := dvector.cons h t
+local notation `[` l:(foldr `, ` (h t, dvector.cons h t) dvector.nil `]`:0) := l
 
+def Set_structure_fun_map : Π {n : ℕ}, L_ZFC.functions n → dvector Set n → Set := λ n f,
+begin
+  cases f,
+    { exact λ _, Set.empty },
+    { intro z, cases z, refine Set.pair z_x _, cases z_xs, exact z_xs_x },
+    { exact λ _, Set.omega },
+    { intro z, cases z, exact Set.powerset z_x },
+    { intro z, cases z, exact Set.Union z_x }
+end
 
+def Set_structure_rel_map : Π {n : ℕ}, L_ZFC.relations n → dvector Set n → Prop := λ n f,
+begin
+  cases f, intro z, cases z, refine Set.mem z_x _, cases z_xs, exact z_xs_x
+end
 
+def Set_structure : Structure L_ZFC :=
+ { carrier := Set,
+   fun_map := λ n f, Set_structure_fun_map f,
+   rel_map := λ n R, Set_structure_rel_map R }
+
+local infix ` ∈'`:100 := _root_.mem
+local infix ` ∈ᴾ`:100 := Set.mem
+
+@[simp]
+lemma realize_bounded_formula_mem {n} {v : dvector Set_structure n} (t₁ t₂ : bounded_term L_ZFC n) :
+  realize_bounded_formula v (t₁ ∈' t₂) ([]) =
+  realize_bounded_term v t₁ ([]) ∈ᴾ realize_bounded_term v t₂ ([]) := rfl
+
+lemma Set_models_extensionality : Set_structure ⊨ axiom_of_extensionality :=
+begin
+  simp[ssatisfied, axiom_of_extensionality], exact λ _ _ H_ext, Set.ext H_ext
+end
+
+theorem Set_ZFC : Set_structure ⊨ ZFC :=
+begin
+  intros ϕ Hϕ, repeat {auto_cases}; try {subst Hϕ},
+    { sorry },
+    { sorry },
+    { sorry },
+    { sorry },
+    { sorry },
+    { exact Set_models_extensionality },
+    { sorry },
+    { sorry },
+    { sorry }
+end
